wip

deps/poulet4/lib/P4automata/WPSymLeap.v
@@ -108,8 +108,8 @@ Section WeakestPreSymbolicLeap.
   Definition wp (phi: conf_rel S H) : list (conf_rel S H) :=
     let cur_st_left  := phi.(cr_st).(cs_st1) in
     let cur_st_right := phi.(cr_st).(cs_st2) in
-    let pred_pairs := list_prod (max_preds Left ([inr false; inr true] ++ List.map (fun s => inl (inl s)) (enum S1)) cur_st_left)
-                                (max_preds Right ([inr false; inr true] ++ List.map (fun s => inl (inr s)) (enum S2)) cur_st_right) in
+    let pred_pairs := list_prod (max_preds Left (List.map (fun s => inl (inl s)) (enum S1)) cur_st_left)
+                                (max_preds Right (List.map (fun s => inl (inr s)) (enum S2)) cur_st_right) in
     List.concat (List.map (wp_pred_pair phi) pred_pairs).
 
 End WeakestPreSymbolicLeap.
